examples/diningcryptos/extra_boolScript.sml
@@ -6,7 +6,8 @@ val _ = new_theory "extra_bool";
 (* Definitions.                                                              *)
 (* ------------------------------------------------------------------------- *)
 
-val xor_def = Define `xor (x:bool) y = ~(x = y)`;val _ = set_fixity "xor" (Infixr 750);
+val xor_def = Define `xor (x:bool) y = ~(x = y)`;
+val _ = set_fixity "xor" (Infixr 750);
 
 (* ------------------------------------------------------------------------- *)
 (* Theorems.                                                                 *)
@@ -32,6 +33,51 @@ val CONJ_EQ_IMP = store_thm
    ``!a b c. (a ==> (b = c)) ==> (a /\ b = a /\ c)``,
    PROVE_TAC []);
 
-(* ------------------------------------------------------------------------- *)val xor_comm = store_thm  ("xor_comm",   ``!x y. x xor y = y xor x``,   RW_TAC bool_ss [xor_def] THEN DECIDE_TAC);val xor_assoc = store_thm  ("xor_assoc",   ``!x y z. (x xor y) xor z = x xor (y xor z)``,   RW_TAC bool_ss [xor_def] THEN DECIDE_TAC);val xor_F = store_thm  ("xor_F",   ``!x. x xor F = x``,   RW_TAC bool_ss [xor_def]);val xor_F = store_thm  ("xor_F",   ``!x. F xor x = x``,   RW_TAC bool_ss [xor_def]);val xor_T = store_thm  ("xor_T",   ``!x. x xor T = ~x``,   RW_TAC bool_ss [xor_def]);val T_xor = store_thm  ("T_xor",   ``!x. T xor x = ~x``,   RW_TAC bool_ss [xor_def]);val xor_refl = store_thm  ("xor_refl",   ``!x. ~(x xor x)``,   RW_TAC bool_ss [xor_def]);val xor_inv = store_thm  ("xor_inv",   ``!x. x xor ~x``,   RW_TAC bool_ss [xor_def] THEN DECIDE_TAC);val inv_xor = store_thm  ("inv_xor",   ``!x. ~x xor x``,   RW_TAC bool_ss [xor_def] THEN DECIDE_TAC);
+(* ------------------------------------------------------------------------- *)
+
+val xor_comm = store_thm
+  ("xor_comm",
+   ``!x y. x xor y = y xor x``,
+   RW_TAC bool_ss [xor_def] THEN DECIDE_TAC);
+
+val xor_assoc = store_thm
+  ("xor_assoc",
+   ``!x y z. (x xor y) xor z = x xor (y xor z)``,
+   RW_TAC bool_ss [xor_def] THEN DECIDE_TAC);
+
+val xor_F = store_thm
+  ("xor_F",
+   ``!x. x xor F = x``,
+   RW_TAC bool_ss [xor_def]);
+
+val xor_F = store_thm
+  ("xor_F",
+   ``!x. F xor x = x``,
+   RW_TAC bool_ss [xor_def]);
+
+val xor_T = store_thm
+  ("xor_T",
+   ``!x. x xor T = ~x``,
+   RW_TAC bool_ss [xor_def]);
+
+val T_xor = store_thm
+  ("T_xor",
+   ``!x. T xor x = ~x``,
+   RW_TAC bool_ss [xor_def]);
+
+val xor_refl = store_thm
+  ("xor_refl",
+   ``!x. ~(x xor x)``,
+   RW_TAC bool_ss [xor_def]);
+
+val xor_inv = store_thm
+  ("xor_inv",
+   ``!x. x xor ~x``,
+   RW_TAC bool_ss [xor_def] THEN DECIDE_TAC);
+
+val inv_xor = store_thm
+  ("inv_xor",
+   ``!x. ~x xor x``,
+   RW_TAC bool_ss [xor_def] THEN DECIDE_TAC);
 
 val _ = export_theory ();
