examples/diningcryptos/extra_realScript.sml
@@ -1,11 +1,11 @@
 (* interactive mode
 loadPath := ["../ho_prover","../subtypes","../rsa"] @ !loadPath;
 app load ["bossLib","realLib","transcTheory","subtypeTheory",
-          "formalizeUseful","extra_boolTheory",
+          "hurdUtils","extra_boolTheory",
           "boolContext","extra_pred_setTools","sumTheory"];
 
 open HolKernel Parse boolLib bossLib realTheory realLib
-     formalizeUseful subtypeTheory extra_numTheory transcTheory
+     hurdUtils subtypeTheory extra_numTheory transcTheory
      pred_setTheory arithmeticTheory seqTheory combinTheory pairTheory
      extra_pred_setTheory extra_boolTheory extra_pred_setTools
      sumTheory;
@@ -13,14 +13,14 @@ open HolKernel Parse boolLib bossLib realTheory realLib
 
 loadPath := ["../subtypes"] @ !loadPath;
 app load ["bossLib","realLib","transcTheory","subtypeTheory",
-          "formalizeUseful","extra_boolTheory",
+          "hurdUtils","extra_boolTheory",
           "extra_pred_setTheory","sumTheory"];
 
 quietdec := true;
 *)
 
 open HolKernel Parse boolLib bossLib realTheory realLib
-     formalizeUseful subtypeTheory extra_numTheory transcTheory
+     hurdUtils subtypeTheory extra_numTheory transcTheory
      pred_setTheory arithmeticTheory seqTheory combinTheory pairTheory
      extra_pred_setTheory extra_boolTheory real_sigmaTheory
      sumTheory limTheory listTheory rich_listTheory;
