examples/miller/formalize/extra_listScript.sml
@@ -21,7 +21,7 @@ val () = app load
 val () = show_assums := true;
 *)
 
-open bossLib listTheory numTheory arithmeticTheory HurdUseful
+open bossLib listTheory numTheory arithmeticTheory hurdUtils
      pred_setTheory subtypeTheory extra_numTheory rich_listTheory;
 
 infixr 0 ++ << || THENC ORELSEC ORELSER ##;
