examples/miller/groups/extra_binomialScript.sml
@@ -29,7 +29,7 @@ installPP subtypeTools.pp_context;
 
 open bossLib arithmeticTheory dividesTheory gcdTheory
      res_quanTheory pred_setTheory subtypeTheory
-     res_quanTools subtypeTools ho_proverTools numContext HurdUseful
+     res_quanTools subtypeTools ho_proverTools numContext hurdUtils
      extra_numTheory ho_basicTools arithContext extra_arithTheory
      binomialTheory summationTheory;
 
