src/probability/martingaleScript.sml
@@ -1,0 +1,540 @@
+(* ------------------------------------------------------------------------- *)
+(* The theory of martingales for sigma-finite measure spaces                 *)
+(*                                                                           *)
+(* Author: Chun Tian (2019)                                                  *)
+(* Fondazione Bruno Kessler and University of Trento, Italy                  *)
+(* ------------------------------------------------------------------------- *)
+
+open HolKernel Parse boolLib bossLib;
+
+open pairTheory relationTheory optionTheory prim_recTheory arithmeticTheory
+     pred_setTheory combinTheory realTheory realLib seqTheory transcTheory
+     real_sigmaTheory posetTheory;
+
+open hurdUtils util_probTheory extrealTheory sigma_algebraTheory measureTheory
+     borelTheory lebesgueTheory;
+
+val _ = new_theory "martingale";
+
+(* "The theory of martingales as we know it now goes back to
+    Doob and most of the material of this and the following chapter can be found in
+    his seminal monograph [2] from 1953.
+
+    We want to understand martingales as an analysis tool which will be useful
+    for the study of L^p- and almost everywhere convergence and, in particular,
+    for the further development of measure and integration theory. Our presentation
+    differs somewhat from the standard way to introduce martingales - conditional
+    expectations will be defined later in Chapter 22 - but the results and their
+    proofs are pretty much the usual ones."
+
+  -- Rene L. Schilling, "Measures, Integrals and Martingales" [1]
+
+   "Martingale theory illustrates the history of mathematical probability: the
+    basic definitions are inspired by crude notions of gambling, but the theory
+    has become a sophisticated tool of modern abstract mathematics, drawing from
+    and contributing to other field."
+
+  -- J. L. Doob, "What is a Martingale?" [3] *)
+
+(* ------------------------------------------------------------------------- *)
+(*  Basic version of martingales (Chapter 17 of [1])                         *)
+(* ------------------------------------------------------------------------- *)
+
+val sub_sigma_algebra_def = Define
+   `sub_sigma_algebra a b <=> sigma_algebra a /\ sigma_algebra b /\
+                             (space a = space b) /\ (subsets a) SUBSET (subsets b)`;
+
+(* sub_sigma_algebra is a partial-order between sigma-algebras *)
+val SUB_SIGMA_ALGEBRA_REFL = store_thm
+  ("SUB_SIGMA_ALGEBRA_REFL",
+  ``!a. sigma_algebra a ==> sub_sigma_algebra a a``,
+    RW_TAC std_ss [sub_sigma_algebra_def, SUBSET_REFL]);
+
+val SUB_SIGMA_ALGEBRA_TRANS = store_thm
+  ("SUB_SIGMA_ALGEBRA_TRANS",
+  ``!a b c. sub_sigma_algebra a b /\ sub_sigma_algebra b c ==> sub_sigma_algebra a c``,
+    RW_TAC std_ss [sub_sigma_algebra_def]
+ >> MATCH_MP_TAC SUBSET_TRANS
+ >> Q.EXISTS_TAC `subsets b` >> art []);
+
+val SUB_SIGMA_ALGEBRA_ANTISYM = store_thm
+  ("SUB_SIGMA_ALGEBRA_ANTISYM",
+  ``!a b. sub_sigma_algebra a b /\ sub_sigma_algebra b a ==> (a = b)``,
+    RW_TAC std_ss [sub_sigma_algebra_def]
+ >> Q.PAT_X_ASSUM `space b = space a` K_TAC
+ >> ONCE_REWRITE_TAC [GSYM SPACE]
+ >> ASM_REWRITE_TAC [CLOSED_PAIR_EQ]
+ >> MATCH_MP_TAC SUBSET_ANTISYM >> art []);
+
+val SUB_SIGMA_ALGEBRA_ORDER = store_thm
+  ("SUB_SIGMA_ALGEBRA_ORDER", ``Order sub_sigma_algebra``,
+    RW_TAC std_ss [Order, antisymmetric_def, transitive_def]
+ >- (MATCH_MP_TAC SUB_SIGMA_ALGEBRA_ANTISYM >> art [])
+ >> IMP_RES_TAC SUB_SIGMA_ALGEBRA_TRANS);
+
+val SUB_SIGMA_ALGEBRA_MEASURE_SPACE = store_thm
+  ("SUB_SIGMA_ALGEBRA_MEASURE_SPACE",
+  ``!m a. measure_space m /\ sub_sigma_algebra a (m_space m,measurable_sets m) ==>
+          measure_space (m_space m,subsets a,measure m)``,
+    RW_TAC std_ss [sub_sigma_algebra_def, space_def, subsets_def]
+ >> MATCH_MP_TAC MEASURE_SPACE_RESTRICTION
+ >> Q.EXISTS_TAC `measurable_sets m`
+ >> simp [MEASURE_SPACE_REDUCE]
+ >> METIS_TAC [SPACE]);
+
+(* `filtration A` is the set of all filtrations of A *)
+val filtration_def = Define
+   `filtration A (a :num -> 'a algebra) <=>
+      (!n. sub_sigma_algebra (a n) A) /\
+      (!i j. i <= j ==> subsets (a i) SUBSET subsets (a j))`;
+
+val FILTRATION_BOUNDED = store_thm
+  ("FILTRATION_BOUNDED",
+  ``!A a. filtration A a ==> !n. sub_sigma_algebra (a n) A``,
+    PROVE_TAC [filtration_def]);
+
+val FILTRATION_MONO = store_thm
+  ("FILTRATION_MONO",
+  ``!A a. filtration A a ==> !i j. i <= j ==> subsets (a i) SUBSET subsets (a j)``,
+    PROVE_TAC [filtration_def]);
+
+(* all sigma-algebras in `filtration A` are subset of A *)
+val FILTRATION_SUBSETS = store_thm
+  ("FILTRATION_SUBSETS",
+  ``!A a. filtration A a ==> !n. subsets (a n) SUBSET (subsets A)``,
+    RW_TAC std_ss [filtration_def, sub_sigma_algebra_def]);
+
+val FILTRATION = store_thm
+  ("FILTRATION",
+  ``!A a. filtration A a <=> (!n. sub_sigma_algebra (a n) A) /\
+                             (!n. subsets (a n) SUBSET (subsets A)) /\
+                             (!i j. i <= j ==> subsets (a i) SUBSET subsets (a j))``,
+    rpt GEN_TAC >> EQ_TAC
+ >- (DISCH_TAC >> IMP_RES_TAC FILTRATION_SUBSETS >> fs [filtration_def])
+ >> RW_TAC std_ss [filtration_def]);
+
+val filtered_measure_space_def = Define
+   `filtered_measure_space (sp,sts,m) a <=>
+             measure_space (sp,sts,m) /\ filtration (sp,sts) a`;
+
+val filtered_measure_space_alt = store_thm
+  ("filtered_measure_space_alt",
+  ``!m a. filtered_measure_space m a <=>
+          measure_space m /\ filtration (m_space m,measurable_sets m) a``,
+    rpt GEN_TAC
+ >> Cases_on `m` >> Cases_on `r`
+ >> REWRITE_TAC [filtered_measure_space_def, m_space_def, measurable_sets_def]);
+
+(* `sigma_finite_FMS = sigma_finite_filtered_measure_space` *)
+val sigma_finite_FMS_def = Define
+   `sigma_finite_FMS (sp,sts,m) a <=>
+    filtered_measure_space (sp,sts,m) a /\ sigma_finite (sp,subsets (a 0),m)`;
+
+val sigma_finite_FMS_alt = store_thm
+  ("sigma_finite_FMS_alt",
+  ``!m a. sigma_finite_FMS m a <=>
+          filtered_measure_space m a /\ sigma_finite (m_space m,subsets (a 0),measure m)``,
+    rpt GEN_TAC
+ >> Cases_on `m` >> Cases_on `r`
+ >> REWRITE_TAC [sigma_finite_FMS_def, m_space_def, measure_def]);
+
+(* all sub measure spaces of a sigma-finite fms are also sigma-finite *)
+val SIGMA_FINITE_FMS_IMP = store_thm
+  ("SIGMA_FINITE_FMS_IMP",
+  ``!sp sts a m. sigma_finite_FMS (sp,sts,m) a ==> !n. sigma_finite (sp,subsets (a n),m)``,
+ (* proof *)
+    RW_TAC std_ss [sigma_finite_FMS_def, filtered_measure_space_def, filtration_def]
+ >> Know `measure_space (sp,subsets (a 0),m) /\
+          measure_space (sp,subsets (a n),m)`
+ >- (CONJ_TAC \\ (* 2 subgoals, same tactics *)
+     MATCH_MP_TAC
+       (REWRITE_RULE [m_space_def, measurable_sets_def, measure_def]
+                     (Q.SPEC `(sp,sts,m)` SUB_SIGMA_ALGEBRA_MEASURE_SPACE)) >> art [])
+ >> STRIP_TAC
+ >> POP_ASSUM (simp o wrap o (MATCH_MP SIGMA_FINITE_ALT))
+ >> POP_ASSUM (fs o wrap o (MATCH_MP SIGMA_FINITE_ALT))
+ >> Q.EXISTS_TAC `f`
+ >> fs [IN_FUNSET, IN_UNIV, measurable_sets_def, m_space_def, measure_def]
+ >> `0 <= n` by RW_TAC arith_ss []
+ >> METIS_TAC [SUBSET_DEF]);
+
+(* extended definition *)
+val SIGMA_FINITE_FMS = store_thm
+  ("SIGMA_FINITE_FMS",
+  ``!sp sts a m. sigma_finite_FMS (sp,sts,m) a <=>
+                 filtered_measure_space (sp,sts,m) a /\
+                 !n. sigma_finite (sp,subsets (a n),m)``,
+    rpt GEN_TAC >> EQ_TAC
+ >- (DISCH_TAC >> IMP_RES_TAC SIGMA_FINITE_FMS_IMP \\
+     fs [sigma_finite_FMS_def])
+ >> RW_TAC std_ss [sigma_finite_FMS_def]);
+
+(* the smallest sigma-algebra generated by all (a n) *)
+val infty_sigma_algebra_def = Define
+   `infty_sigma_algebra sp a = sigma sp (BIGUNION (IMAGE (\(i :num). subsets (a i)) UNIV))`;
+
+val INFTY_SIGMA_ALGEBRA_BOUNDED = store_thm
+  ("INFTY_SIGMA_ALGEBRA_BOUNDED",
+  ``!A a. filtration A a ==>
+          sub_sigma_algebra (infty_sigma_algebra (space A) a) A``,
+    RW_TAC std_ss [sub_sigma_algebra_def, FILTRATION, infty_sigma_algebra_def]
+ >- (MATCH_MP_TAC SIGMA_ALGEBRA_SIGMA \\
+     RW_TAC std_ss [subset_class_def, IN_BIGUNION_IMAGE, IN_UNIV] \\
+    `x IN subsets A` by PROVE_TAC [SUBSET_DEF] \\
+     METIS_TAC [sigma_algebra_def, algebra_def, subset_class_def, space_def, subsets_def])
+ >- REWRITE_TAC [SPACE_SIGMA]
+ >> MATCH_MP_TAC SIGMA_SUBSET >> art []
+ >> RW_TAC std_ss [SUBSET_DEF, IN_BIGUNION_IMAGE, IN_UNIV]
+ >> PROVE_TAC [SUBSET_DEF]);
+
+val INFTY_SIGMA_ALGEBRA_MAXIMAL = store_thm
+  ("INFTY_SIGMA_ALGEBRA_MAXIMAL",
+  ``!A a. filtration A a ==> !n. sub_sigma_algebra (a n) (infty_sigma_algebra (space A) a)``,
+ (* proof *)
+    RW_TAC std_ss [sub_sigma_algebra_def, FILTRATION, infty_sigma_algebra_def]
+ >- (MATCH_MP_TAC SIGMA_ALGEBRA_SIGMA \\
+     RW_TAC std_ss [subset_class_def, IN_BIGUNION_IMAGE, IN_UNIV] \\
+    `x IN subsets A` by PROVE_TAC [SUBSET_DEF] \\
+     METIS_TAC [sigma_algebra_def, algebra_def, subset_class_def, space_def, subsets_def])
+ >- REWRITE_TAC [SPACE_SIGMA]
+ >> MATCH_MP_TAC SUBSET_TRANS
+ >> Q.EXISTS_TAC `BIGUNION (IMAGE (\i. subsets (a i)) univ(:num))`
+ >> CONJ_TAC
+ >- (RW_TAC std_ss [SUBSET_DEF, IN_BIGUNION_IMAGE, IN_UNIV] \\
+     Q.EXISTS_TAC `n` >> art [])
+ >> REWRITE_TAC [SIGMA_SUBSET_SUBSETS]);
+
+(* `prob_martingale` will be the probability version of `martingale` *)
+val martingale_def = Define
+   `martingale m a u <=>
+      sigma_finite_FMS m a /\ (!n. integrable m (u n)) /\
+      !n s. s IN (subsets (a n)) ==>
+           (integral m (\x. u (SUC n) x * indicator_fn s x) =
+            integral m (\x. u n x * indicator_fn s x))`;
+
+(* super-martingale: changed `=` with `<=` *)
+val super_martingale_def = Define
+   `super_martingale m a u <=>
+      sigma_finite_FMS m a /\ (!n. integrable m (u n)) /\
+      !n s. s IN (subsets (a n)) ==>
+           (integral m (\x. u (SUC n) x * indicator_fn s x) <=
+            integral m (\x. u n x * indicator_fn s x))`;
+
+(* sub-martingale: integral (u n) <= integral (u (SUC n)), looks more natural *)
+val sub_martingale_def = Define
+   `sub_martingale m a u <=>
+      sigma_finite_FMS m a /\ (!n. integrable m (u n)) /\
+      !n s. s IN (subsets (a n)) ==>
+           (integral m (\x. u n x * indicator_fn s x) <=
+            integral m (\x. u (SUC n) x * indicator_fn s x))`;
+
+(* u is a martingale if, and only if, it is both a sub- and a supermartingale *)
+val MARTINGALE_BOTH_SUB_SUPER = store_thm
+  ("MARTINGALE_BOTH_SUB_SUPER",
+  ``!m a u. martingale m a u <=> sub_martingale m a u /\ super_martingale m a u``,
+    RW_TAC std_ss [martingale_def, sub_martingale_def, super_martingale_def]
+ >> EQ_TAC >> RW_TAC std_ss [le_refl]
+ >> ASM_SIMP_TAC std_ss [GSYM le_antisym]);
+
+(* ------------------------------------------------------------------------- *)
+(*  General version of martingales with poset indexes (Chapter 19 of [1])    *)
+(* ------------------------------------------------------------------------- *)
+
+val POSET_NUM_LE = store_thm
+  ("POSET_NUM_LE", ``poset (univ(:num),$<=)``,
+    RW_TAC std_ss [poset_def]
+ >- (Q.EXISTS_TAC `0` >> REWRITE_TAC [GSYM IN_APP, IN_UNIV])
+ >- (MATCH_MP_TAC LESS_EQUAL_ANTISYM >> art [])
+ >> MATCH_MP_TAC LESS_EQ_TRANS
+ >> Q.EXISTS_TAC `y` >> art []);
+
+(* below J is an index set, R is a partial order on J *)
+val general_filtration_def = Define
+   `general_filtration A a (J,R) <=>
+      poset (J,R) /\ (!n. n IN J ==> sub_sigma_algebra (a n) A) /\
+      (!i j. i IN J /\ j IN J /\ R i j ==> subsets (a i) SUBSET subsets (a j))`;
+
+val TO_GENERAL_FILTRATION = store_thm
+  ("TO_GENERAL_FILTRATION",
+  ``!A a. filtration A a = general_filtration A a (univ(:num),$<=)``,
+    RW_TAC std_ss [filtration_def, general_filtration_def, POSET_NUM_LE, IN_UNIV]);
+
+val general_fms_def = Define
+   `general_fms (sp,sts,m) a (J,R) <=>
+             measure_space (sp,sts,m) /\ general_filtration (sp,sts) a (J,R)`;
+
+val general_fms_alt = store_thm
+  ("general_fms_alt",
+  ``!sp sts m a. filtered_measure_space (sp,sts,m) a <=>
+                 general_fms (sp,sts,m) a (univ(:num),$<=)``,
+    RW_TAC std_ss [filtered_measure_space_def, general_fms_def,
+                   TO_GENERAL_FILTRATION, POSET_NUM_LE, IN_UNIV]);
+
+val sigma_finite_general_fms_def = Define
+   `sigma_finite_general_fms (sp,sts,m) a (J,R) <=>
+          general_fms (sp,sts,m) a (J,R) /\
+          !n. n IN J ==> sigma_finite (sp,subsets (a n),m)`;
+
+val SIGMA_FINITE_FMS_SIGMA_FINITE_FMS_I = store_thm
+  ("SIGMA_FINITE_FMS_SIGMA_FINITE_FMS_I",
+  ``!sp sts m a. sigma_finite_FMS (sp,sts,m) a <=>
+                 sigma_finite_general_fms (sp,sts,m) a (univ(:num),$<=)``,
+    RW_TAC std_ss [SIGMA_FINITE_FMS, sigma_finite_general_fms_def,
+                   general_fms_alt, IN_UNIV]);
+
+val infty_sigma_algebra_I_def = Define
+   `infty_sigma_algebra_I sp a I = sigma sp (BIGUNION (IMAGE (\i. subsets (a i)) I))`;
+
+(* `general_martingale m a u (univ(:num),$<=) = martingale m a u` *)
+val general_martingale_def = Define
+   `general_martingale m a u (J,R) <=>
+      sigma_finite_general_fms m a (J,R) /\ (!n. n IN J ==> integrable m (u n)) /\
+      !i j s. i IN J /\ j IN J /\ R i j /\ s IN (subsets (a i)) ==>
+             (integral m (\x. u i x * indicator_fn s x) =
+              integral m (\x. u j x * indicator_fn s x))`;
+
+(* or "upwards directed" *)
+val upwards_filtering_def = Define
+   `upwards_filtering (J,R) <=> !a b. a IN J /\ b IN J ==> ?c. c IN J /\ R a c /\ R b c`;
+
+(* The smallest sigma-algebra on `sp` that makes `f` measurable *)
+val sigma_function_def = Define
+   `sigma_function sp A f = (sp,IMAGE (\s. PREIMAGE f s INTER sp) (subsets A))`;
+
+val _ = overload_on ("sigma", ``sigma_function``);
+
+val SIGMA_MEASURABLE = store_thm
+  ("SIGMA_MEASURABLE",
+  ``!sp A f. sigma_algebra A /\ f IN (sp -> space A) ==> f IN measurable (sigma sp A f) A``,
+    RW_TAC std_ss [sigma_function_def, space_def, subsets_def,
+                   IN_FUNSET, IN_MEASURABLE, IN_IMAGE]
+ >- (MATCH_MP_TAC PREIMAGE_SIGMA_ALGEBRA >> art [IN_FUNSET])
+ >> Q.EXISTS_TAC `s` >> art []);
+
+(* Definition 7.5 of [1, p.51], The smallest sigma-algebra on `sp` that makes all `f`
+   simultaneously measurable. *)
+val sigma_functions_def = Define
+   `sigma_functions sp A f J =
+      sigma sp (BIGUNION (IMAGE (\i. IMAGE (\s. PREIMAGE (f i) s INTER sp) (subsets (A i))) J))`;
+
+val _ = overload_on ("sigma", ``sigma_functions``);
+
+(* Lemma 7.5 of [1, p.51] *)
+val SIGMA_SIMULTANEOUSLY_MEASURABLE = store_thm
+  ("SIGMA_SIMULTANEOUSLY_MEASURABLE",
+  ``!sp A f J. (!i. i IN J ==> sigma_algebra (A i)) /\
+               (!i. f i IN (sp -> space (A i))) ==>
+                !i. i IN J ==> f i IN measurable (sigma sp A f J) (A i)``,
+    RW_TAC std_ss [IN_FUNSET, SPACE_SIGMA, sigma_functions_def, IN_MEASURABLE]
+ >- (MATCH_MP_TAC SIGMA_ALGEBRA_SIGMA \\
+     RW_TAC std_ss [subset_class_def, IN_BIGUNION_IMAGE, IN_IMAGE, IN_PREIMAGE, IN_INTER] \\
+     REWRITE_TAC [INTER_SUBSET])
+ >> Know `PREIMAGE (f i) s INTER sp IN
+            (BIGUNION (IMAGE (\i. IMAGE (\s. PREIMAGE (f i) s INTER sp) (subsets (A i))) J))`
+ >- (RW_TAC std_ss [IN_BIGUNION_IMAGE, IN_IMAGE] \\
+     Q.EXISTS_TAC `i` >> art [] \\
+     Q.EXISTS_TAC `s` >> art []) >> DISCH_TAC
+ >> ASSUME_TAC
+      (Q.SPECL [`sp`, `BIGUNION (IMAGE (\i. IMAGE (\s. PREIMAGE (f i) s INTER sp)
+                                                  (subsets (A i))) J)`] SIGMA_SUBSET_SUBSETS)
+ >> PROVE_TAC [SUBSET_DEF]);
+
+(* ------------------------------------------------------------------------- *)
+(* Some prelimitaries of Radon-Nikodym Theorem                               *)
+(* ------------------------------------------------------------------------- *)
+
+Definition seq_sup_def :
+  (seq_sup P 0       = @r. r IN P /\ sup P < r + 1) /\
+  (seq_sup P (SUC n) = @r. r IN P /\ sup P < r + Normal ((1 / 2) pow (SUC n)) /\
+                           (seq_sup P n) < r /\ r < sup P)
+End
+
+val EXTREAL_SUP_SEQ = store_thm
+  ("EXTREAL_SUP_SEQ",
+  ``!P. (?x. P x) /\ (?z. z <> PosInf /\ !x. P x ==> x <= z) ==>
+        ?x. (!n. x n IN P) /\ (!n. x n <= x (SUC n)) /\ (sup (IMAGE x UNIV) = sup P)``,
+  RW_TAC std_ss []
+  >> Cases_on `?z. P z /\ (z = sup P)`
+  >- (Q.EXISTS_TAC `(\i. sup P)`
+      >> RW_TAC std_ss [le_refl,SPECIFICATION]
+      >> `IMAGE (\i:num. sup P) UNIV = (\i. i = sup P)`
+           by RW_TAC std_ss [EXTENSION,IN_IMAGE,IN_UNIV,IN_ABS]
+      >> RW_TAC std_ss [sup_const])
+  >> Cases_on `!x. P x ==> (x = NegInf)`
+  >- (`sup P = NegInf` by METIS_TAC [sup_const_alt]
+      >> Q.EXISTS_TAC `(\n. NegInf)`
+      >> FULL_SIMP_TAC std_ss [le_refl]
+      >> RW_TAC std_ss []
+      >- METIS_TAC []
+      >> METIS_TAC [UNIV_NOT_EMPTY,sup_const_over_set])
+  >> FULL_SIMP_TAC std_ss []
+  >> Q.EXISTS_TAC `seq_sup P`
+  >> FULL_SIMP_TAC std_ss []
+  >> `sup P <> PosInf` by METIS_TAC [sup_le,lt_infty,let_trans]
+  >> `!x. P x ==> x < sup P` by METIS_TAC [lt_le,le_sup_imp]
+  >> `!e. 0 < e ==> ?x. P x /\ sup P < x + e`
+       by (RW_TAC std_ss [] >> MATCH_MP_TAC sup_lt_epsilon >> METIS_TAC [])
+  >> `!n. 0:real < (1 / 2) pow n` by METIS_TAC [HALF_POS,REAL_POW_LT]
+  >> `!n. 0 < Normal ((1 / 2) pow n)` by METIS_TAC [extreal_lt_eq,extreal_of_num_def]
+  >> `!n. seq_sup P n IN P`
+      by (Induct
+          >- (RW_TAC std_ss [seq_sup_def]
+              >> SELECT_ELIM_TAC
+              >> RW_TAC std_ss []
+              >> METIS_TAC [lt_01,SPECIFICATION])
+          >> RW_TAC std_ss [seq_sup_def]
+          >> SELECT_ELIM_TAC
+          >> RW_TAC std_ss []
+          >> `?x. P x /\ seq_sup P n < x` by METIS_TAC [sup_lt,SPECIFICATION]
+          >> `?x. P x /\ sup P < x + Normal ((1 / 2) pow (SUC n))` by METIS_TAC []
+          >> Q.EXISTS_TAC `max x'' x'''`
+          >> RW_TAC std_ss [extreal_max_def,SPECIFICATION]
+          >- (`x''' < x''` by FULL_SIMP_TAC std_ss [GSYM extreal_lt_def]
+              >> `x''' +  Normal ((1 / 2) pow (SUC n)) <= x'' +  Normal ((1 / 2) pow (SUC n))`
+                  by METIS_TAC [lt_radd,lt_le,extreal_not_infty]
+              >> METIS_TAC [lte_trans])
+          >> METIS_TAC [lte_trans])
+  >> `!n. seq_sup P n <= seq_sup P (SUC n)`
+      by (RW_TAC std_ss [seq_sup_def]
+          >> SELECT_ELIM_TAC
+          >> RW_TAC std_ss []
+          >- (`?x. P x /\ seq_sup P n < x` by METIS_TAC [sup_lt,SPECIFICATION]
+              >> `?x. P x /\ sup P < x + Normal ((1 / 2) pow (SUC n))` by METIS_TAC []
+              >> Q.EXISTS_TAC `max x'' x'''`
+              >> RW_TAC std_ss [extreal_max_def,SPECIFICATION]
+              >- (`x''' < x''` by FULL_SIMP_TAC std_ss [GSYM extreal_lt_def]
+                  >> `x''' + Normal ((1 / 2) pow (SUC n)) <= x'' + Normal ((1 / 2) pow (SUC n))`
+                      by METIS_TAC [lt_radd,lt_le,extreal_not_infty]
+                  >> METIS_TAC [lte_trans])
+              >> METIS_TAC [lte_trans])
+          >> METIS_TAC [lt_le])
+  >> RW_TAC std_ss []
+  >> `!n. sup P <= seq_sup P n + Normal ((1 / 2) pow n)`
+      by (Induct
+          >- (RW_TAC std_ss [seq_sup_def,pow,GSYM extreal_of_num_def]
+              >> SELECT_ELIM_TAC
+              >> RW_TAC std_ss []
+              >- METIS_TAC [lt_01,SPECIFICATION]
+              >> METIS_TAC [lt_le])
+          >> RW_TAC std_ss [seq_sup_def]
+          >> SELECT_ELIM_TAC
+          >> RW_TAC std_ss []
+          >- (`?x. P x /\ seq_sup P n < x` by METIS_TAC [sup_lt,SPECIFICATION]
+              >> `?x. P x /\ sup P < x + Normal ((1 / 2) pow (SUC n))` by METIS_TAC []
+              >> Q.EXISTS_TAC `max x'' x'''`
+              >> RW_TAC std_ss [extreal_max_def,SPECIFICATION]
+              >- (`x''' < x''` by FULL_SIMP_TAC std_ss [GSYM extreal_lt_def]
+                  >> `x''' + Normal ((1 / 2) pow (SUC n)) <= x'' + Normal ((1 / 2) pow (SUC n))`
+                      by METIS_TAC [lt_radd,lt_le,extreal_not_infty]
+                  >> METIS_TAC [lte_trans])
+              >> METIS_TAC [lte_trans])
+          >> METIS_TAC [lt_le])
+  >> RW_TAC std_ss [sup_eq]
+  >- (POP_ASSUM (MP_TAC o ONCE_REWRITE_RULE [GSYM SPECIFICATION])
+      >> RW_TAC std_ss [IN_IMAGE,IN_UNIV]
+      >> METIS_TAC [SPECIFICATION,lt_le])
+  >> MATCH_MP_TAC le_epsilon
+  >> RW_TAC std_ss []
+  >> `e <> NegInf` by METIS_TAC [lt_infty,extreal_of_num_def,lt_trans]
+  >> `?r. e = Normal r` by METIS_TAC [extreal_cases]
+  >> FULL_SIMP_TAC std_ss []
+  >> `?n. Normal ((1 / 2) pow n) < Normal r` by METIS_TAC [EXTREAL_ARCH_POW_INV]
+  >> MATCH_MP_TAC le_trans
+  >> Q.EXISTS_TAC `seq_sup P n + Normal ((1 / 2) pow n)`
+  >> RW_TAC std_ss []
+  >> MATCH_MP_TAC le_add2
+  >> FULL_SIMP_TAC std_ss [lt_le]
+  >> Q.PAT_X_ASSUM `!z. IMAGE (seq_sup P) UNIV z ==> z <= y` MATCH_MP_TAC
+  >> ONCE_REWRITE_TAC [GSYM SPECIFICATION]
+  >> RW_TAC std_ss [IN_UNIV,IN_IMAGE]
+  >> METIS_TAC []);
+
+val EXTREAL_SUP_FUN_SEQ_IMAGE = store_thm
+  ("EXTREAL_SUP_FUN_SEQ_IMAGE",
+  ``!(P:extreal->bool) (P':('a->extreal)->bool) f.
+       (?x. P x) /\ (?z. z <> PosInf /\ !x. P x ==> x <= z) /\ (P = IMAGE f P')
+           ==> ?g. (!n:num. g n IN P') /\
+                   (sup (IMAGE (\n. f (g n)) UNIV) = sup P)``,
+  rpt STRIP_TAC
+  >> `?y. (!n. y n IN P) /\ (!n. y n <= y (SUC n)) /\ (sup (IMAGE y UNIV) = sup P)`
+     by METIS_TAC [EXTREAL_SUP_SEQ]
+  >> Q.EXISTS_TAC `(\n. @r. (r IN P') /\ (f r  = y n))`
+  >> `(\n. f (@(r :'a -> extreal). r IN (P' :('a -> extreal) -> bool) /\
+                                  ((f :('a -> extreal) -> extreal) r = (y :num -> extreal) n))) = y`
+  by (rw [FUN_EQ_THM] >> SELECT_ELIM_TAC
+      >> RW_TAC std_ss []
+      >> METIS_TAC [IN_IMAGE])
+  >> ASM_SIMP_TAC std_ss []
+  >> RW_TAC std_ss []
+  >- (SELECT_ELIM_TAC
+      >> RW_TAC std_ss []
+      >> METIS_TAC [IN_IMAGE]));
+
+val max_fn_seq_def = Define `
+   (max_fn_seq g 0 x  = g 0 x) /\
+   (max_fn_seq g (SUC n) x = max (max_fn_seq g n x) (g (SUC n) x))`;
+
+val max_fn_seq_mono = store_thm
+  ("max_fn_seq_mono", ``!g n x. max_fn_seq g n x <= max_fn_seq g (SUC n) x``,
+    RW_TAC std_ss [max_fn_seq_def,extreal_max_def,le_refl]);
+
+val EXTREAL_SUP_FUN_SEQ_MONO_IMAGE = store_thm
+  ("EXTREAL_SUP_FUN_SEQ_MONO_IMAGE",
+  ``!f (P:extreal->bool) (P':('a->extreal)->bool).
+                (?x. P x) /\ (?z. z <> PosInf /\ !x. P x ==> x <= z) /\ (P = IMAGE f P') /\
+                (!g1 g2. (g1 IN P' /\ g2 IN P' /\ (!x. g1 x <= g2 x))  ==> f g1 <= f g2) /\
+                (!g1 g2. g1 IN P' /\ g2 IN P' ==> (\x. max (g1 x) (g2 x)) IN P')
+          ==> ?g. (!n. g n IN P') /\
+                  (!x n. g n x <= g (SUC n) x) /\
+                  (sup (IMAGE (\n. f (g n)) UNIV) = sup P)``,
+  rpt STRIP_TAC
+  >> `?g. (!n:num. g n IN P') /\ (sup (IMAGE (\n. f (g n)) UNIV) = sup P)`
+      by METIS_TAC [EXTREAL_SUP_FUN_SEQ_IMAGE]
+  >> Q.EXISTS_TAC `max_fn_seq g`
+  >> `!n. max_fn_seq g n IN P'`
+      by (Induct
+          >- (`max_fn_seq g 0 = g 0` by RW_TAC std_ss [FUN_EQ_THM,max_fn_seq_def]
+              >> METIS_TAC [])
+              >> `max_fn_seq g (SUC n) = (\x. max (max_fn_seq g n x) (g (SUC n) x))`
+                  by RW_TAC std_ss [FUN_EQ_THM,max_fn_seq_def]
+              >> RW_TAC std_ss []
+              >> METIS_TAC [])
+  >> `!g n x. max_fn_seq g n x <= max_fn_seq g (SUC n) x`
+      by RW_TAC real_ss [max_fn_seq_def,extreal_max_def,le_refl]
+  >> CONJ_TAC >- RW_TAC std_ss []
+  >> CONJ_TAC >- RW_TAC std_ss []
+  >> `!n. (!x. g n x <= max_fn_seq g n x)`
+      by (Induct >- RW_TAC std_ss [max_fn_seq_def,le_refl]
+          >> METIS_TAC [le_max2,max_fn_seq_def])
+  >> `!n. f (g n) <= f (max_fn_seq g n)` by METIS_TAC []
+  >> `sup (IMAGE (\n. f (g n)) UNIV) <= sup (IMAGE (\n. f (max_fn_seq g n)) UNIV)`
+      by (MATCH_MP_TAC sup_le_sup_imp
+          >> RW_TAC std_ss []
+          >> POP_ASSUM (MP_TAC o ONCE_REWRITE_RULE [GSYM SPECIFICATION])
+          >> RW_TAC std_ss [IN_IMAGE,IN_UNIV]
+          >> Q.EXISTS_TAC `f (max_fn_seq g n)`
+          >> RW_TAC std_ss []
+          >> ONCE_REWRITE_TAC [GSYM SPECIFICATION]
+          >> RW_TAC std_ss [IN_IMAGE,IN_UNIV]
+          >> METIS_TAC [])
+  >> `sup (IMAGE (\n. f (max_fn_seq g n)) UNIV) <= sup P`
+      by (RW_TAC std_ss [sup_le]
+          >> POP_ASSUM (MP_TAC o ONCE_REWRITE_RULE [GSYM SPECIFICATION])
+          >> RW_TAC std_ss [IN_IMAGE,IN_UNIV]
+          >> MATCH_MP_TAC le_sup_imp
+          >> ONCE_REWRITE_TAC [GSYM SPECIFICATION]
+          >> RW_TAC std_ss [IN_IMAGE]
+          >> METIS_TAC [])
+  >> METIS_TAC [le_antisym]);
+
+val _ = export_theory ();
+val _ = html_theory "martingale";
+
+(* References:
+
+  [1] Schilling, R.L.: Measures, Integrals and Martingales (Second Edition).
+      Cambridge University Press (2017).
+  [2] Doob, J.L.: Stochastic processes. Wiley-Interscience (1990).
+  [3] Doob, J.L.: What is a Martingale? Amer. Math. Monthly. 78(5), 451-463 (1971).
+  [4] Pintacuda, N.: Probabilita'. Zanichelli, Bologna (1995).
+ *)
